% ======================================
% Proof: PL-SUP-C08-EX02A-T17-01
% ======================================
\clearpage
\phantomsection
\hypertarget{proof-PL-SUP-C08-EX02A-T17-01}{}

\section*{Proof — PL-SUP-C08-EX02A-T17-01}

\noindent
\hyperlink{ws-PL-SUP-C08-EX02A-T17-01}{\textbf{← Back to worksheet}}

\noindent
\textbf{Source.}
\srccite{SuppesHillFirstCourseLogic}{Chapter~8, Exercise~2(A)}.

\vspace{0.75em}

\noindent
\textbf{Goal.} Prove $(\forall x)(\forall y)(\forall z)(\forall w)((x-y=z-w)\leftrightarrow(x+w=y+z))$.

\vspace{0.75em}

\noindent
\textbf{Proof (stub).}
\[
\begin{array}{r l l}
(1) &  &  \\
(2) &  &  \\
(3) &  &  \\
(4) &  &  \\
(5) &  &  \\
(6) &  &  \\
(7) &  &
\end{array}
\]

\vspace{1em}
\noindent
\hyperlink{ws-PL-SUP-C08-EX02A-T17-01}{\textbf{← Back to worksheet}}
