% ======================================
% Proof: PL-SUP-C06-S6.1-E03-01
% ======================================
\clearpage
\phantomsection
\hypertarget{proof-PL-SUP-C06-S6.1-E03-01}{}

\section*{Proof — PL-SUP-C06-S6.1-E03-01}

\noindent
\hyperlink{ws-PL-SUP-C06-S6.1-E03-01}{\textbf{← Back to worksheet}}

\noindent
\textbf{Source.}
\srccite{SuppesHillFirstCourseLogic}{Chapter~6, \S6.1}.

\vspace{0.75em}

\noindent
\textbf{Goal.} Derive $Ga$.

\vspace{0.75em}

\noindent
\textbf{Given (Premises).}
\[
\begin{array}{r l l}
(1) & (\forall x)(Hx \rightarrow Gx) & \text{P} \\
(2) & Ha & \text{P}
\end{array}
\]

\vspace{0.75em}

\noindent
\textbf{Proof (stub).}
\[
\begin{array}{r l l}
(1) & (\forall x)(Hx \rightarrow Gx) & \text{P} \\
(2) & Ha & \text{P} \\
(3) & (Ha \rightarrow Ga & \text{Universal Specification} \\
(4) & Ga) & \text{Modus Ponens} \\

\end{array}
\]

\vspace{1em}

\noindent
\hyperlink{ws-PL-SUP-C06-S6.1-E03-01}{\textbf{← Back to worksheet}}