% ======================================
% Proof: PL-SUP-C02-S2.2-P03
% ======================================
\clearpage
\phantomsection
\hypertarget{proof-PL-SUP-C02-S2.2-P03}{}

\section*{Proof â€” PL-SUP-C02-S2.2-P03}

}

\noindent
\textbf{Source.}
\srccite{SuppesHillFirstCourseLogic}{Chapter~2, \S2}.

\vspace{0.75em}

\noindent
\textbf{Goal.} Prove $C$.

\vspace{0.75em}

\noindent
\textbf{Given (Premises).}
\[
\begin{array}{r l l}
(1) & A \rightarrow (B \wedge D) & \text{P} \\
(2) & (B \wedge D) \rightarrow C & \text{P} \\
(3) & A & \text{P} \\
\end{array}
\]

\vspace{0.75em}

\noindent
\textbf{Proof (stub).}
\[
\begin{array}{r l l}
(1) & A \rightarrow (B \wedge D) & \text{P} \\
(2) & (B \wedge D) \rightarrow C & \text{P} \\
(3) & A & \text{P} \\
(4) & (B \wedge D) & \text{MP} \\
(5) & C & \text{MP} \\
\end{array}
\]

\vspace{0.75em}

\noindent
\textbf{Remarks.}
\begin{itemize}
  \item Target: $C$.
  \item Keep each derived line justified by a named rule (e.g., detachment, etc.).
\end{itemize}

\vspace{1em}

}