% ======================================
% Proof: PL-SUP-C02-S2.5-E03
% ======================================
\clearpage
\phantomsection
\hypertarget{proof-PL-SUP-C02-S2.5-E03}{}

\section*{Proof â€” PL-SUP-C02-S2.5-E03}

}

\noindent
\textbf{Source.}
\srccite{SuppesHillFirstCourseLogic}{Chapter~2, \S2.5}.

\vspace{0.75em}

\noindent
\textbf{Goal.} Prove $Q$.

\vspace{0.75em}

\noindent
\textbf{Given (Premises).}
\[
\begin{array}{r l l}
(1) & \neg R \rightarrow S & \text{P} \\
(2) & S \rightarrow (P \wedge Q) & \text{P} \\
(3) & R \rightarrow T & \text{P} \\
(4) & \neg T & \text{P} \\
\end{array}
\]

\vspace{0.75em}

\noindent
\textbf{Proof (stub).}
\[
\begin{array}{r l l}
(1) & \neg R \rightarrow S & \text{P} \\
(2) & S \rightarrow (P \wedge Q) & \text{P} \\
(3) & R \rightarrow T & \text{P} \\
(4) & \neg T & \text{P} \\
(5) & \neg R & \text{MT} \\
(6) & S & \text{MP} \\
(7) & (P \wedge Q) & \text{MP} \\
(8) & Q & \text{Rule of Simplification} \\

\end{array}
\]

\vspace{1em}

}