% ======================================
% Proof: PL-SUP-C03-S3.6-E10-06
% ======================================
\clearpage
\phantomsection
\hypertarget{proof-PL-SUP-C03-S3.6-E10-06}{}

\section*{Proof â€” PL-SUP-C03-S3.6-E10-06}

}

\noindent
\textbf{Source.}
\srccite{SuppesHillFirstCourseLogic}{Chapter~3, \S3.6}.

\vspace{0.75em}

\noindent
\textbf{Goal.} Derive a contradiction ($\bot$) from the premises (show the set is inconsistent).

\vspace{0.75em}

\noindent
\textbf{Given (Premises).}
\[
\begin{array}{r l l}
(1) & x = 1 \rightarrow y < x & \text{P} \\
(2) & y < x \rightarrow y = 0 & \text{P} \\
(3) & \neg (y = 0 \vee x \neq 1) & \text{P}
\end{array}
\]

\vspace{0.75em}

\noindent
\textbf{Proof (stub).}
\[
\begin{array}{r l l}
(1) & x = 1 \rightarrow y < x & \text{P} \\
(2) & y < x \rightarrow y = 0 & \text{P} \\
(3) & \neg (y = 0 \vee x \neq 1) & \text{P} \\
(4) &  &  \\
(5) &  &  \\
(6) &  &  \\
(7) &  & 
\end{array}
\]

\vspace{1em}

}