\begin{proof}
We prove left cancellation; right cancellation is symmetric.
Assume $ab = ac$ for $a, b, c \in G$.

\noindent
\begin{tabular}{T S J}
\toprule
\textbf{Tag} & \multicolumn{1}{p{0.44\textwidth}}{\textbf{Step}} & \textbf{Justification} \\
\midrule
\addlinespace[4pt]

\tagDU
&
a^{-1} \in G
&
Every element of $G$ has an inverse (Axiom G3).
\\[10pt]

\tagAM
&
a^{-1}(ab) = a^{-1}(ac)
&
Multiply both sides of $ab = ac$ on the left by $a^{-1}$.
\\[10pt]

\tagTA
&
(a^{-1}a)b = (a^{-1}a)c
&
Associativity (Axiom G1) applied to both sides.
\\[10pt]

\tagDU
&
eb = ec
&
$a^{-1}a = e$ by definition of inverse (Axiom G3).
\\[10pt]

\tagDU
&
b = c
&
$ea = a$ for all $a \in G$ by definition of identity (Axiom G2).
\hfill$\blacksquare$
\\[6pt]

\bottomrule
\end{tabular}

\medskip
\noindent Right cancellation follows by the symmetric argument,
multiplying on the right by $a^{-1}$.
\end{proof}