\subsection{Suppes}

\noindent
\textbf{Source.}
Patrick Suppes and Shirley Hill
\textit{First Course in Mathematical Logic},
Chapter 1 (selected exercises).

\vspace{0.5em}

\begin{longtable}{|p{4.5cm}|p{8.5cm}|}
\hline
\textbf{Problem ID} & \textbf{Exercise (descriptor)} \\
\hline
\endfirsthead
\hline
\textbf{Problem ID} & \textbf{Exercise (descriptor)} \\
\hline
\endhead
\hline
\endfoot
\hline
\endlastfoot

\hline
\hypertarget{ws-PL-SUP-C02-S2.2-P03}{%
\hyperlink{proof-PL-SUP-C02-S2.2-P03}{\texttt{PL-SUP-C02-S2.2-P03}}}
&
Prove $C$ from $A \rightarrow (B \wedge D)$, $(B \wedge D) \rightarrow C$, and $A$
(Suppes \& Hill, Ch.~2, \S2.2, Problem~3).
\\ \hline

\hypertarget{ws-PL-SUP-C02-S2.2-P04}{%
\hyperlink{proof-PL-SUP-C02-S2.2-P04}{\texttt{PL-SUP-C02-S2.2-P04}}}
&
Prove $M \vee N$ from $\neg J \rightarrow (M \vee N)$, $(F \vee G) \rightarrow \neg J$,
and $F \vee G$
(Suppes \& Hill, Ch.~2, \S2.2, Problem~4).
\\ \hline

\hypertarget{ws-PL-SUP-C02-S2.2-P05}{%
\hyperlink{proof-PL-SUP-C02-S2.2-P05}{\texttt{PL-SUP-C02-S2.2-P05}}}
&
Prove $\neg S$ from $T$, $T \rightarrow \neg Q$, and $\neg Q \rightarrow \neg S$
(Suppes \& Hill, Ch.~2, \S2.2, Problem~5).
\\ \hline

\hypertarget{ws-PL-SUP-C02-S2.3-P02}{%
\hyperlink{proof-PL-SUP-C02-S2.3-P02}{\texttt{PL-SUP-C02-S2.3-P02}}}
&
Prove $B$ from $\neg A$ and $\neg A \rightarrow \neg\neg B$
(Suppes \& Hill, Ch.~2, \S2.3, Problem~2).
\\ \hline

\hypertarget{ws-PL-SUP-C02-S2.3-P03}{%
\hyperlink{proof-PL-SUP-C02-S2.3-P03}{\texttt{PL-SUP-C02-S2.3-P03}}}
&
Prove $G$ from $H \rightarrow \neg\neg G$ and $H$
(Suppes \& Hill, Ch.~2, \S2.3, Problem~3).
\\ \hline

\hypertarget{ws-PL-SUP-C02-S2.3-P04}{%
\hyperlink{proof-PL-SUP-C02-S2.3-P04}{\texttt{PL-SUP-C02-S2.3-P04}}}
&
Prove $P \vee Q$ from $R \rightarrow \neg\neg(P \vee Q)$ and $R$
(Suppes \& Hill, Ch.~2, \S2.3, Problem~4).
\\ \hline

\hypertarget{ws-PL-SUP-C02-S2.3-P06}{%
\hyperlink{proof-PL-SUP-C02-S2.3-P06}{\texttt{PL-SUP-C02-S2.3-P06}}}
&
Prove $Q$ from $J \rightarrow (K \wedge M)$, $J$, and $(K \wedge M) \rightarrow \neg\neg Q$
(Suppes \& Hill, Ch.~2, \S2.3, Problem~6).
\\ \hline

\hypertarget{ws-PL-SUP-C02-S2.5-E01}{%
\hyperlink{proof-PL-SUP-C02-S2.5-E01}{\texttt{PL-SUP-C02-S2.5-E01}}}
&
Prove $\neg T$ from $(Q \rightarrow R)\wedge P$, $R \rightarrow T$, and $(Q \rightarrow R)\rightarrow \neg T$
(Suppes \& Hill, Ch.~2, \S2.5, Exercise~1).
\\ \hline

\hypertarget{ws-PL-SUP-C02-S2.5-E02}{%
\hyperlink{proof-PL-SUP-C02-S2.5-E02}{\texttt{PL-SUP-C02-S2.5-E02}}}
&
Prove $P$ from $\neg R$, $\neg P \rightarrow Q$, and $Q \rightarrow R$
(Suppes \& Hill, Ch.~2, \S2.5, Exercise~2).
\\ \hline

\hypertarget{ws-PL-SUP-C02-S2.5-E03}{%
\hyperlink{proof-PL-SUP-C02-S2.5-E03}{\texttt{PL-SUP-C02-S2.5-E03}}}
&
Prove $Q$ from $\neg R \rightarrow S$, $S \rightarrow (P \wedge Q)$, $R \rightarrow T$, and $\neg T$
(Suppes \& Hill, Ch.~2, \S2.5, Exercise~3).
\\ \hline

\hypertarget{ws-PL-SUP-C02-S2.5-E06}{%
\hyperlink{proof-PL-SUP-C02-S2.5-E06}{\texttt{PL-SUP-C02-S2.5-E06}}}
&
Prove $\neg T$ from $T \rightarrow (P \wedge S)$, $Q \rightarrow \neg P$, $R \rightarrow \neg S$, and $R \vee Q$
(Suppes \& Hill, Ch.~2, \S2.5, Exercise~6).
\\ \hline

\hypertarget{ws-PL-SUP-C02-S2.5-E07}{%
\hyperlink{proof-PL-SUP-C02-S2.5-E07}{\texttt{PL-SUP-C02-S2.5-E07}}}
&
Prove $\neg P$ from $R \rightarrow \neg P$, $(R \wedge S)\vee T$, $T \rightarrow (Q \vee U)$, and $\neg Q \wedge \neg U$
(Suppes \& Hill, Ch.~2, \S2.5, Exercise~7).
\\ \hline

\hypertarget{ws-PL-SUP-C02-S2.5-E08}{%
\hyperlink{proof-PL-SUP-C02-S2.5-E08}{\texttt{PL-SUP-C02-S2.5-E08}}}
&
Prove $R \wedge Q$ from $P \vee Q$, $S \rightarrow (Q \wedge R)$, $P \rightarrow S$, and $Q \rightarrow S$
(Suppes \& Hill, Ch.~2, \S2.5, Exercise~8).
\\ \hline

\hypertarget{ws-PL-SUP-C02-S2.5-E09}{%
\hyperlink{proof-PL-SUP-C02-S2.5-E09}{\texttt{PL-SUP-C02-S2.5-E09}}}
&
Prove $G \vee \neg H$ from $(E \vee F)\rightarrow \neg H$, $J \rightarrow E$, $K \rightarrow F$, and $J \vee K$
(Suppes \& Hill, Ch.~2, \S2.5, Exercise~9).
\\ \hline

\hypertarget{ws-PL-SUP-C02-S2.5-E10}{%
\hyperlink{proof-PL-SUP-C02-S2.5-E10}{\texttt{PL-SUP-C02-S2.5-E10}}}
&
Prove $S \wedge T$ from $\neg(P \vee \neg R)$, $Q \vee P$, $R \rightarrow S$, and $(Q \wedge S)\rightarrow (T \wedge S)$
(Suppes \& Hill, Ch.~2, \S2.5, Exercise~10).
\\ \hline

% ------------------------------------------------------------
% ADDITIONAL WORKSHEET ENTRIES — Suppes, Ch. 3, §3.6, Ex. 10
% (Append these rows inside the existing longtable, before \end{longtable}.)
% ------------------------------------------------------------

\hypertarget{ws-PL-SUP-C03-S3.6-E10-01}{%
\hyperlink{proof-PL-SUP-C03-S3.6-E10-01}{\texttt{PL-SUP-C03-S3.6-E10-01}}}
&
Derive a contradiction ($\bot$) from $\neg Q \rightarrow R$, $\neg R \vee S$, $\neg(P \vee Q)$, and $\neg P \rightarrow \neg S$
(Suppes \& Hill, Ch.~3, \S3.6, Exercise~10.1).
\\ \hline

\hypertarget{ws-PL-SUP-C03-S3.6-E10-02}{%
\hyperlink{proof-PL-SUP-C03-S3.6-E10-02}{\texttt{PL-SUP-C03-S3.6-E10-02}}}
&
Derive a contradiction ($\bot$) from $T \rightarrow P$, $T \wedge R$, $Q \rightarrow \neg R$, and $(P \vee S) \rightarrow Q$
(Suppes \& Hill, Ch.~3, \S3.6, Exercise~10.2).
\\ \hline

\hypertarget{ws-PL-SUP-C03-S3.6-E10-03}{%
\hyperlink{proof-PL-SUP-C03-S3.6-E10-03}{\texttt{PL-SUP-C03-S3.6-E10-03}}}
&
Derive a contradiction ($\bot$) from $R \rightarrow (R \wedge Q)$, $\neg S \vee R$, $\neg T \vee \neg Q$, and $S \wedge T$
(Suppes \& Hill, Ch.~3, \S3.6, Exercise~10.3).
\\ \hline

\hypertarget{ws-PL-SUP-C03-S3.6-E10-04}{%
\hyperlink{proof-PL-SUP-C03-S3.6-E10-04}{\texttt{PL-SUP-C03-S3.6-E10-04}}}
&
Derive a contradiction ($\bot$) from $T \vee \neg R$, $\neg(R \rightarrow S)$, and $T \rightarrow S$
(Suppes \& Hill, Ch.~3, \S3.6, Exercise~10.4).
\\ \hline

\hypertarget{ws-PL-SUP-C03-S3.6-E10-05}{%
\hyperlink{proof-PL-SUP-C03-S3.6-E10-05}{\texttt{PL-SUP-C03-S3.6-E10-05}}}
&
Derive a contradiction ($\bot$) from $Q \rightarrow P$, $\neg(P \vee R)$, and $Q \vee R$
(Suppes \& Hill, Ch.~3, \S3.6, Exercise~10.5).
\\ \hline

\hypertarget{ws-PL-SUP-C03-S3.6-E10-06}{%
\hyperlink{proof-PL-SUP-C03-S3.6-E10-06}{\texttt{PL-SUP-C03-S3.6-E10-06}}}
&
Derive a contradiction ($\bot$) from $x = 1 \rightarrow y < x$, $y < x \rightarrow y = 0$, and $\neg(y = 0 \vee x \neq 1)$
(Suppes \& Hill, Ch.~3, \S3.6, Exercise~10.6).
\\ \hline



















\end{longtable}
