% =========================================================
% Worksheet: Suppes & Hill — Predicate Calculus
% File: predicate-calculus/worksheets/suppes.tex
% =========================================================

\subsection{Suppes \& Hill}

\noindent\textbf{Source.} Suppes \& Hill, \textit{First Course in Mathematical Logic}.

\vspace{0.75em}
\begin{center}
\begin{tabular}{|p{5.0cm}|p{9.0cm}|}
\hline
\textbf{Problem ID} & \textbf{Exercise (descriptor)} \\
\hline

% -------------------------
% Chapter 6, §6.1
% -------------------------
\phantomsection
\hypertarget{ws-PL-SUP-C06-S6.1-E03-01}{}
\hyperlink{proof-PL-SUP-C06-S6.1-E03-01}{\texttt{PL-SUP-C06-S6.1-E03-01}}
&
Suppes \& Hill, Chapter 6, \S6.1 — Derive $Ga$.
\\ \hline

\phantomsection
\hypertarget{ws-PL-SUP-C06-S6.1-E07-01}{}
\hyperlink{proof-PL-SUP-C06-S6.1-E07-01}{\texttt{PL-SUP-C06-S6.1-E07-01}}
&
Suppes \& Hill, Chapter 6, \S6.1 — Derive $\neg Hf$.
\\ \hline

\phantomsection
\hypertarget{ws-PL-SUP-C06-S6.1-E09-01}{}
\hyperlink{proof-PL-SUP-C06-S6.1-E09-01}{\texttt{PL-SUP-C06-S6.1-E09-01}}
&
Suppes \& Hill, Chapter 6, \S6.1 — Derive $Jb$.
\\ \hline

\phantomsection
\hypertarget{ws-PL-SUP-C06-S6.1-E10-01}{}
\hyperlink{proof-PL-SUP-C06-S6.1-E10-01}{\texttt{PL-SUP-C06-S6.1-E10-01}}
&
Suppes \& Hill, Chapter 6, \S6.1 — Derive $Hx$.
\\ \hline

% -------------------------
% Chapter 7 — Axioms (Symbolization)
% -------------------------
\phantomsection
\hypertarget{ws-PL-SUP-C07-A01}{}
\hyperlink{proof-PL-SUP-C07-A01}{\texttt{PL-SUP-C07-A01}}
&
Suppes \& Hill, Chapter 7 — Commutative Axiom for addition (symbolized).
\\ \hline

\phantomsection
\hypertarget{ws-PL-SUP-C07-A02}{}
\hyperlink{proof-PL-SUP-C07-A02}{\texttt{PL-SUP-C07-A02}}
&
Suppes \& Hill, Chapter 7 — Associative Axiom for addition (symbolized).
\\ \hline

\phantomsection
\hypertarget{ws-PL-SUP-C07-A03}{}
\hyperlink{proof-PL-SUP-C07-A03}{\texttt{PL-SUP-C07-A03}}
&
Suppes \& Hill, Chapter 7 — Axiom for Zero (additive identity, symbolized).
\\ \hline

\phantomsection
\hypertarget{ws-PL-SUP-C07-A04}{}
\hyperlink{proof-PL-SUP-C07-A04}{\texttt{PL-SUP-C07-A04}}
&
Suppes \& Hill, Chapter 7 — Axiom for Negative Numbers (additive inverses, symbolized).
\\ \hline

% -------------------------
% Chapter 8 — Exercise 2(A)
% -------------------------

\phantomsection
\hypertarget{ws-PL-SUP-C08-EX02A-T07-01}{}
\hyperlink{proof-PL-SUP-C08-EX02A-T07-01}{\texttt{PL-SUP-C08-EX02A-T07-01}}
&
Suppes \& Hill, Chapter 8, Ex.~2(A) — $(\forall x)(0-x=-x)$.
\\ \hline

\phantomsection
\hypertarget{ws-PL-SUP-C08-EX02A-T08-01}{}
\hyperlink{proof-PL-SUP-C08-EX02A-T08-01}{\texttt{PL-SUP-C08-EX02A-T08-01}}
&
Suppes \& Hill, Chapter 8, Ex.~2(A) — $(x-y)+(y-z)=x-z$.
\\ \hline

\phantomsection
\hypertarget{ws-PL-SUP-C08-EX02A-T09-01}{}
\hyperlink{proof-PL-SUP-C08-EX02A-T09-01}{\texttt{PL-SUP-C08-EX02A-T09-01}}
&
Suppes \& Hill, Chapter 8, Ex.~2(A) — $(-x=y)\rightarrow(x=-y)$.
\\ \hline

\phantomsection
\hypertarget{ws-PL-SUP-C08-EX02A-T10-01}{}
\hyperlink{proof-PL-SUP-C08-EX02A-T10-01}{\texttt{PL-SUP-C08-EX02A-T10-01}}
&
Suppes \& Hill, Chapter 8, Ex.~2(A) — $(x+y=z+y)\rightarrow(x=z)$.
\\ \hline

\phantomsection
\hypertarget{ws-PL-SUP-C08-EX02A-T11-01}{}
\hyperlink{proof-PL-SUP-C08-EX02A-T11-01}{\texttt{PL-SUP-C08-EX02A-T11-01}}
&
Suppes \& Hill, Chapter 8, Ex.~2(A) — $(-y+-x)+(x+y)=0$.
\\ \hline

\phantomsection
\hypertarget{ws-PL-SUP-C08-EX02A-T12-01}{}
\hyperlink{proof-PL-SUP-C08-EX02A-T12-01}{\texttt{PL-SUP-C08-EX02A-T12-01}}
&
Suppes \& Hill, Chapter 8, Ex.~2(A) — $-(x+y)=(-x)+(-y)$.
\\ \hline

\phantomsection
\hypertarget{ws-PL-SUP-C08-EX02A-T13-01}{}
\hyperlink{proof-PL-SUP-C08-EX02A-T13-01}{\texttt{PL-SUP-C08-EX02A-T13-01}}
&
Suppes \& Hill, Chapter 8, Ex.~2(A) — $(x-y)+(z-w)=(x+z)-(y+w)$.
\\ \hline

\phantomsection
\hypertarget{ws-PL-SUP-C08-EX02A-T14-01}{}
\hyperlink{proof-PL-SUP-C08-EX02A-T14-01}{\texttt{PL-SUP-C08-EX02A-T14-01}}
&
Suppes \& Hill, Chapter 8, Ex.~2(A) — $(x-y)-(z-w)=(x+w)-(y+z)$.
\\ \hline

\phantomsection
\hypertarget{ws-PL-SUP-C08-EX02A-T15-01}{}
\hyperlink{proof-PL-SUP-C08-EX02A-T15-01}{\texttt{PL-SUP-C08-EX02A-T15-01}}
&
Suppes \& Hill, Chapter 8, Ex.~2(A) — $(x-y=z)\leftrightarrow(x-z=y)$.
\\ \hline

\phantomsection
\hypertarget{ws-PL-SUP-C08-EX02A-T16-01}{}
\hyperlink{proof-PL-SUP-C08-EX02A-T16-01}{\texttt{PL-SUP-C08-EX02A-T16-01}}
&
Suppes \& Hill, Chapter 8, Ex.~2(A) — $(x+y=z)\leftrightarrow(x-z=-y)$.
\\ \hline

\phantomsection
\hypertarget{ws-PL-SUP-C08-EX02A-T17-01}{}
\hyperlink{proof-PL-SUP-C08-EX02A-T17-01}{\texttt{PL-SUP-C08-EX02A-T17-01}}
&
Suppes \& Hill, Chapter 8, Ex.~2(A) — $(x-y=z-w)\leftrightarrow(x+w=y+z)$.
\\ \hline

\end{tabular}
\end{center}
