\begin{proof}
We show $a \cdot 0 = 0$; the proof that $0 \cdot a = 0$ is symmetric.

\noindent
\begin{tabular}{T S J}
\toprule
\textbf{Tag} & \multicolumn{1}{p{0.44\textwidth}}{\textbf{Step}} & \textbf{Justification} \\
\midrule
\addlinespace[4pt]

\tagDU
&
0 + 0 = 0
&
$0$ is the additive identity (Axiom R1).
\\[10pt]

\tagAM
&
a \cdot 0 = a \cdot (0 + 0)
&
Substituting $0 = 0 + 0$.
\\[10pt]

\tagDU
&
a \cdot (0 + 0) = a \cdot 0 + a \cdot 0
&
Left distributivity (Axiom R3).
\\[10pt]

\tagAM
&
a \cdot 0 + a \cdot 0 = a \cdot 0
&
Combining the chain: $a \cdot 0 = a \cdot 0 + a \cdot 0$.
\\[10pt]

\tagTA
&
a \cdot 0 = 0
&
Add $-(a \cdot 0)$ to both sides.
Left side: $(a \cdot 0 + a \cdot 0) + (-(a \cdot 0)) = a \cdot 0$.
Right side: $a \cdot 0 + (-(a \cdot 0)) = 0$.
By additive cancellation
(Proposition~\ref{prop:group-cancellation}).
\hfill$\blacksquare$
\\[6pt]

\bottomrule
\end{tabular}
\end{proof}
