\begin{proof}
We show $a \cdot (-b) = -(a \cdot b)$;
the proof for $(-a) \cdot b$ is symmetric.

It suffices to show $a \cdot (-b)$ satisfies the defining property
of the additive inverse of $a \cdot b$, then invoke uniqueness.

\noindent
\begin{tabular}{T S J}
\toprule
\textbf{Tag} & \multicolumn{1}{p{0.44\textwidth}}{\textbf{Step}} & \textbf{Justification} \\
\midrule
\addlinespace[4pt]

\tagAM
&
(a \cdot b) + (a \cdot (-b)) = a \cdot (b + (-b))
&
Left distributivity (Axiom R3).
\\[10pt]

\tagDU
&
a \cdot (b + (-b)) = a \cdot 0
&
$b + (-b) = 0$ by definition of additive inverse (Axiom R1).
\\[10pt]

\tagTA
&
a \cdot 0 = 0
&
Proposition~\ref{prop:ring-mult-zero}.
\\[10pt]

\tagDU
&
(a \cdot b) + (a \cdot (-b)) = 0
&
Combining: $a \cdot (-b)$ is an additive inverse of $a \cdot b$.
\\[10pt]

\tagTA
&
a \cdot (-b) = -(a \cdot b)
&
Additive inverses are unique
(Proposition~\ref{prop:group-inverse-unique}).
\hfill$\blacksquare$
\\[6pt]

\bottomrule
\end{tabular}
\end{proof}
