% --------------------------------------
% Proof: AA-GAL-C00-E11
% --------------------------------------
\clearpage
\phantomsection
\hypertarget{proof-AA-GAL-C00-E11}{}

\section*{Proof — AA-GAL-C00-E11}

\noindent
\hyperlink{ws-AA-GAL-C00-E11}{\textbf{← Back to worksheet}}

\noindent
\textbf{Source.}
\srccite{GallianCAA7}{Chapter~0, Exercise~11}.

\vspace{0.75em}

\noindent
\textbf{Goal.}
Let $n > 1$ be a fixed positive integer.
If $a \bmod n = a'$ and $b \bmod n = b'$, prove that
\[
(a+b) \bmod n = (a' + b') \bmod n
\]
and
\[
(ab) \bmod n = (a'b') \bmod n.
\]

\vspace{0.75em}

\noindent

\begin{proof}
Since $a \bmod n = a'$ and $b \bmod n = b'$, by the division algorithm there exist integers $q_1, q_2$ such that
\begin{equation}
    a = q_1 n + a', \quad b = q_2 n + b'. \label{eq:AA-GAL-C00-E11-1}
\end{equation}
Adding these equations gives
\[
a + b = (q_1 + q_2)n + (a' + b').
\]
Therefore, since $n \mid (q_1 + q_2)n$,
\[
(a + b) \bmod n = ((q_1 + q_2)n + (a' + b')) \bmod n = (a' + b') \bmod n.
\]
From \eqref{eq:AA-GAL-C00-E11-1} it follows that
\[
ab = (q_1 n + a')(q_2 n + b') = q_1q_2n^2 + q_1nb' + q_2na' + a'b'.
\]
Since $n \mid q_1q_2n^2$, $n \mid q_1nb'$, and $n \mid q_2na'$, we have
\[
(ab) \bmod n = (a'b') \bmod n. \qedhere
\]
\end{proof}

\vspace{2cm}
\noindent
\hyperlink{ws-AA-GAL-C00-E11}{\textbf{← Back to worksheet}}
